Replace old proof with new one

demo/mutrec/MutrecABproof.v
@@ -102,330 +102,379 @@ Section LXSIM.
     admit "ez".
   Qed.
 
-  Inductive match_focus: mem -> Z -> Z -> list Frame.t -> Prop :=
+  Inductive match_focus: mem -> int -> int -> list Frame.t -> Prop :=
+  | match_focus_nil
+      cur max m
+      (OVER: cur.(Int.intval) > max.(Int.intval))
+    :
+      match_focus m cur max []
   | match_focus_cons_A
-      cur max m i tl_tgt
-      (VAL: i.(Int.intval) = cur)
-      (REC: match_focus m (cur + 1)%Z max tl_tgt \/ cur = max)
+      cur max m tl_tgt
+      (REC: match_focus m (Int.add cur Int.one) max tl_tgt)
     :
-      match_focus m cur max ((Frame.mk (MutrecAspec.modsem skenv_link tt) (MutrecAspec.Callstate i m)) :: tl_tgt)
+      match_focus m cur max ((Frame.mk (MutrecAspec.modsem skenv_link tt) (MutrecAspec.Callstate cur m)) :: tl_tgt)
   | match_focus_cons_B
-      cur max m i tl_tgt
-      (VAL: i.(Int.intval) = cur)
-      (REC: match_focus m (cur + 1)%Z max tl_tgt \/ cur = max)
+      cur max m tl_tgt
+      (REC: match_focus m (Int.add cur Int.one) max tl_tgt)
     :
-      match_focus m cur max ((Frame.mk (MutrecBspec.modsem skenv_link tt) (MutrecBspec.Callstate i m)) :: tl_tgt)
+      match_focus m cur max ((Frame.mk (MutrecBspec.modsem skenv_link tt) (MutrecBspec.Callstate cur m)) :: tl_tgt)
   .
 
-  Inductive match_stacks: Z -> list Frame.t -> list Frame.t -> Prop :=
-  | match_stacks_nil
+  Lemma match_focus_over_nil
+        m max hds_tgt
+        (FOCUS: match_focus m (Int.add max Int.one) max hds_tgt)
     :
-      match_stacks 0%Z [] []
-  (* | match_stacks_cons_ctx *)
-  (*     i tail_src tail_tgt *)
-  (*     (TAIL: match_stacks i tail_src tail_tgt) *)
-  (*     hd *)
-  (*   : *)
-  (*     match_stacks 0%Z (hd :: tail_src) (hd :: tail_tgt) *)
+      hds_tgt = nil
+  .
+  Proof.
+    admit "not true now. -- we should know it does not overflow, then it is trivial".
+  Qed.
+
+  Inductive match_stacks (fromcall: bool) (idx: Z): list Frame.t -> list Frame.t -> Prop :=
   | match_stacks_ctx
       ctx_stk
+      (IDX: idx = 0%Z)
     :
-      match_stacks 0%Z ctx_stk ctx_stk
-  | match_stacks_focus
-      (* j tail_src tail_tgt *)
-      (* (TAIL: match_stacks j tail_src tail_tgt) *)
+      match_stacks fromcall idx ctx_stk ctx_stk
+  (* | match_stacks_focus_top_call *)
+  (*     ctx_stk *)
+  (*     cur max m hd_src hds_tgt *)
+  (*     (SRC: hd_src = Frame.mk (MutrecABspec.modsem skenv_link tt) (MutrecABspec.Callstate max m)) *)
+  (*     (LE: (cur <= max.(Int.intval))%Z) *)
+  (*     (TGT: match_focus m cur max.(Int.intval) hds_tgt) *)
+  (*   : *)
+  (*     match_stacks cur (hd_src :: ctx_stk) (hds_tgt ++ ctx_stk) *)
+  | match_stacks_focus_top_call
       ctx_stk
       cur max m hd_src hds_tgt
       (SRC: hd_src = Frame.mk (MutrecABspec.modsem skenv_link tt) (MutrecABspec.Callstate max m))
-      (* (VAL: i.(Int.intval) = max) *)
-      (LE: (cur <= max.(Int.intval))%Z)
-      (TGT: match_focus m cur max.(Int.intval) hds_tgt)
+      hd_tgt
+      (TGT: __GUARD__ ((hd_tgt = Frame.mk (MutrecAspec.modsem skenv_link tt) (MutrecAspec.Callstate cur m)) \/
+                       (hd_tgt = Frame.mk (MutrecBspec.modsem skenv_link tt) (MutrecBspec.Callstate cur m))))
+      (LE: (cur.(Int.intval) <= max.(Int.intval))%Z)
+      (FOCUS: match_focus m (Int.add cur Int.one) max hds_tgt)
+      (* (IDX: idx = (max.(Int.intval) + cur.(Int.intval)) + 1) *)
+      (IDX: idx = cur.(Int.intval))
     :
-      match_stacks cur (hd_src :: ctx_stk) (hds_tgt ++ ctx_stk)
+      match_stacks fromcall idx (hd_src :: ctx_stk) (hd_tgt :: hds_tgt ++ ctx_stk)
+  | match_stacks_focus_top_return
+      ctx_stk
+      cur max m hd_src hds_tgt
+      (SRC: hd_src = Frame.mk (MutrecABspec.modsem skenv_link tt) (MutrecABspec.Returnstate (sum max) m))
+      hd_tgt
+      (TGT: __GUARD__ ((hd_tgt = Frame.mk (MutrecAspec.modsem skenv_link tt) (MutrecAspec.Returnstate (sum cur) m)) \/
+                       (hd_tgt = Frame.mk (MutrecBspec.modsem skenv_link tt) (MutrecBspec.Returnstate (sum cur) m))))
+      (LE: (cur.(Int.intval) <= max.(Int.intval))%Z)
+      (FOCUS: match_focus m (Int.add cur Int.one) max hds_tgt)
+      (FROMCALL: fromcall = false)
+      (IDX: idx = max.(Int.intval) - cur.(Int.intval))
+    :
+      match_stacks fromcall idx (hd_src :: ctx_stk) (hd_tgt :: hds_tgt ++ ctx_stk)
   .
 
   Inductive match_states (i: Z): Sem.state -> Sem.state -> Prop :=
-  | match_states_call_from_ctx
-      args ctx_stk
-    :
-      match_states i (Callstate args ctx_stk) (Callstate args ctx_stk)
-  | match_states_call_from_focus
+  | match_states_call
       frs_src frs_tgt
-      args blk
-      (FOCUS: Genv.find_symbol skenv_link f_id = Some blk \/ Genv.find_symbol skenv_link g_id = Some blk)
-      (FPTR: args.(Args.fptr) = Vptr blk Ptrofs.zero)
-      (STK: match_stacks i frs_src frs_tgt)
+      args
+      (STK: match_stacks true i frs_src frs_tgt)
+      (* blk *)
+      (* (FPTR: args.(Args.fptr) = Vptr blk Ptrofs.zero) *)
+      (* (NFOCUS: ~(Genv.find_symbol skenv_link f_id = Some blk \/ Genv.find_symbol skenv_link g_id = Some blk) -> frs_src = frs_tgt) *)
+      (* (FOCUS: (Genv.find_symbol skenv_link f_id = Some blk \/ Genv.find_symbol skenv_link g_id = Some blk) -> match_stacks i frs_src frs_tgt) *)
     :
       match_states i (Callstate args frs_src) (Callstate args frs_tgt)
   | match_states_normal
       frs_src frs_tgt
-      (STK: match_stacks i frs_src frs_tgt)
+      (STK: match_stacks false i frs_src frs_tgt)
     :
       match_states i (State frs_src) (State frs_tgt)
   .
+
+  Lemma int_zero_intval: Int.intval Int.zero = 0%Z.
+  Proof. unfold Int.intval. ss. Qed.
+
+  Lemma int_sub_add: forall cur x, (Int.add (Int.sub cur x) x) = cur.
+  Proof.
+    i.
+    rewrite Int.sub_add_opp. rewrite Int.add_assoc.
+    rewrite Int.add_commut with (y := x).
+    rewrite Int.add_neg_zero. rewrite Int.add_zero. ss.
+  Qed.
 
   Lemma match_states_xsim
         i st_src0 st_tgt0
         (MATCH: match_states i st_src0 st_tgt0)
     :
       xsim (sem (ctx ++ [module])) (sem (ctx ++ [MutrecAspec.module; MutrecBspec.module]))
-           Z.lt i st_src0 st_tgt0
+           (Zwf.Zwf 0) i st_src0 st_tgt0
   .
   Proof.
     revert_until LINKTGT. pcofix CIH. i.
     inv MATCH.
-    - (* call from ctx *)
-      pfold. right. econs; et.
-      { i; ss. des_ifs. inv FINALTGT. }
-      i.
-      econs; et; cycle 1.
-      + i. specialize (SAFESRC _ (star_refl _ _ _ _)). desH SAFESRC; ss.
-        * left. inv SAFESRC.
-        * right. des_ifs. inv SAFESRC. inv MSFIND. ss. des; clarify.
-          { esplits; et. econs; et. econs; et. ss. et. }
-          folder.
-          unfold load_modsems in *. rewrite in_map_iff in *. des_safe. rewrite in_app_iff in *. ss; des; clarify.
-          { esplits; et. econs; et. econs; et. ss. right. unfold load_modsems in *. rewrite in_map_iff.
-            esplits; et. rewrite in_app_iff. et. }
-          { apply genv_sim in INTERNAL. des. ss. rr in FOCUS. inv INIT.
-            unfold Genv.find_funct, Genv.find_funct_ptr in *. des_ifs.
-            des; clarify.
-            - esplits; et. econs; et.
-              + econs; et.
-                * ss. right. unfold load_modsems in *. rewrite in_map_iff. esplits; et. 
-                  rewrite in_app_iff. right. left. ss; et.
-                * unfold Genv.find_funct, Genv.find_funct_ptr in *. rewrite Heq1. ss. des_ifs. 
-              + econs; ss; et.
-                admit "ez - genv".
-            - esplits; et. econs; et.
-              + econs; et.
-                * ss. right. unfold load_modsems in *. rewrite in_map_iff. esplits; et. 
-                  rewrite in_app_iff. right. right. ss; et.
-                * unfold Genv.find_funct, Genv.find_funct_ptr in *. rewrite Heq1. ss. des_ifs. 
-              + econs; ss; et.
-                admit "ez - genv".
-          }
-      + i. ss. des_ifs. inv STEPTGT. inv MSFIND. ss.
-        unfold load_modsems in *.
-        des; clarify.
-        { esplits; et.
-          - left. apply plus_one. econs; et. econs; et. ss. et.
-          - right. eapply CIH. econs; et. econs; et.
-        }
-        rewrite in_map_iff in *. des. clarify. rewrite in_app_iff in *. des; clarify.
-        { esplits; et.
-          - left. apply plus_one. econs; et. econs; et. ss. right.
-            unfold load_modsems. rewrite in_map_iff. esplits; et. rewrite in_app_iff. et.
-          - right. eapply CIH. econs; et. econs; et.
-        }
-        { ss. des; clarify; ss; inv INIT.
-          - esplits; et.
-            + left. apply plus_one. econs.
-              * instantiate (1:= modsem skenv_link tt).
-                econs; et.
-                -- ss. right. unfold load_modsems. rewrite in_map_iff. esplits; cycle 1.
-                   { rewrite in_app_iff. right; ss; et. }
-                   ss.
-                -- instantiate (1:= if_sig). apply genv_sim. exists (MutrecAspec.module). esplits; et; rr; et.
-              * econs; et.
-                -- instantiate (1:= if_sig). apply genv_sim. exists (MutrecAspec.module). esplits; et; rr; et.
-            + right. eapply CIH. econs; et.
-              rewrite cons_app with (xhd := {|
-                Frame.ms := flip Mod.modsem (Sk.load_skenv sk_link) MutrecAspec.module;
-                Frame.st := MutrecAspec.Callstate i0 (Args.m args) |}).
-              econs; et.
-              * refl.
-              * econs; et.
-          - esplits; et.
-            + left. apply plus_one. econs.
-              * instantiate (1:= modsem skenv_link tt).
-                econs; et.
-                -- ss. right. unfold load_modsems. rewrite in_map_iff. esplits; cycle 1.
-                   { rewrite in_app_iff. right; ss; et. }
-                   ss.
-                -- instantiate (1:= if_sig). apply genv_sim. exists (MutrecBspec.module). esplits; et; rr; et.
-              * econs; et.
-                -- instantiate (1:= if_sig). apply genv_sim. exists (MutrecBspec.module). esplits; et; rr; et.
-            + right. eapply CIH. econs; et.
-              rewrite cons_app with (xhd := {|
-                Frame.ms := flip Mod.modsem (Sk.load_skenv sk_link) MutrecBspec.module;
-                Frame.st := MutrecBspec.Callstate i0 (Args.m args) |}).
-              econs; et.
-              * refl.
-              * econs; et.
-        }
-    - (* call from focus *)
-      pfold. right.
-      econs; et.
-      { ss. i. inv FINALTGT; ss. }
-      i.
-      econs; et; cycle 1.
-      { i; ss. specialize (SAFESRC _ (star_refl _ _ _ _)). desH SAFESRC; ss.
-        - left. inv SAFESRC.
-        - right. des_ifs. inv SAFESRC.
-          inv MSFIND. ss. desH MODSEM.
-          { esplits; et. econs; et. econs; et. ss; et. }
-          unfold load_modsems in *. rewrite in_map_iff in *. des_safe. clarify.
-          rewrite in_app_iff in *. desH MODSEM0; clarify.
-          { esplits; et. econs; et. econs; et. ss; et. right.
-            unfold load_modsems in *. rewrite in_map_iff in *. esplits; et. rewrite in_app_iff. des; et.
-          }
-          ss. des_safe; clarify.
-          exploit genv_sim; et. i; des_safe. exploit FINDF; et. i; des_safe. rr in FOCUS0.
-          desH FOCUS0; clarify; inv INIT; esplits; et.
-          + econs.
-            * instantiate (1:= MutrecAspec.modsem skenv_link tt). econs; et. ss. right.
-              unfold load_modsems, flip in *; rewrite in_map_iff in *; folder; esplits; et; cycle 1.
-              { rewrite in_app_iff; ss. right. left. et. }
-              ss.
-            * econs; ss; et.
-              admit "ez - revive// TODO: make lemma".
-          + econs.
-            * instantiate (1:= MutrecBspec.modsem skenv_link tt). econs; et. ss. right.
-              unfold load_modsems, flip in *; rewrite in_map_iff in *; folder; esplits; et; cycle 1.
-              { rewrite in_app_iff; ss. right. right. et. }
-              ss.
-            * econs; ss; et.
-              admit "ez - revive// TODO: make lemma".
-      }
-      i. ss. des_ifs. inv STEPTGT. folder.
-      assert(MSFIND0:
-               Ge.find_fptr_owner
-               (load_genv (ctx ++ [MutrecAspec.module; MutrecBspec.module]) skenv_link)
-               (Args.fptr args) (MutrecAspec.modsem skenv_link tt)
-             \/
-             Ge.find_fptr_owner
-               (load_genv (ctx ++ [MutrecAspec.module; MutrecBspec.module]) skenv_link)
-               (Args.fptr args) (MutrecBspec.modsem skenv_link tt)
-            ).
-      { des.
-        - left. econs; ss; et.
-          + right. unfold load_modsems. rewrite in_map_iff. esplits; ss; et; cycle 1.
-            { rewrite in_app_iff. right; left; ss; et. }
-            ss.
-          + rewrite FPTR. ss. des_ifs. eapply find_symbol_find_funct_ptr_A; et.
-        - right. econs; ss; et.
-          + right. unfold load_modsems. rewrite in_map_iff. esplits; ss; et; cycle 1.
-            { rewrite in_app_iff. right; right; ss; et. }
-            ss.
-          + rewrite FPTR. ss. des_ifs. eapply find_symbol_find_funct_ptr_B; et.
-      }
-      inv MSFIND. ss. desH MODSEM; clarify.
-      { (* system *)
-        exfalso. ss. admit "exploit system_disjoint; et".
-        (* unfold System.skenv in *. *)
-        (* inv INIT. esplits; eauto. *)
-        (* + left. apply plus_one. esplits; eauto; cycle 1. *)
-        (*   econs; et. *)
-        (*   { econs; ss; et. } *)
-        (*   econs; et. *)
-        (* + right. eapply CIH; et. econs; et. econs 3; et. *)
-      }
-      unfold load_modsems in *. rewrite in_map_iff in *. desH MODSEM. clarify.
-      clarify.
-      rewrite in_app_iff in *. desH MODSEM0; clarify.
-      { (* ctx *)
-        exfalso. ss. admit "somehow".
-        (* esplits; eauto. *)
-        (* + left. apply plus_one. econs; et. econs; et. ss. right. *)
-        (*   unfold load_modsems in *. rewrite in_map_iff. esplits; et. *)
-        (*   rewrite in_app_iff. ss. et. *)
-        (* + right. eapply CIH; et. econs; et. *)
-        (*   rewrite cons_app with (xtl := frs_tgt). *)
-        (*   econs 3; et. *)
-      }
-      { (* focus *)
-        folder.
-        inv STK.
-        assert(exists i, <<ARGS: Args.vs args = [Vint i]>>).
-        { ss. des; clarify; inv INIT; et. }
-        des.
-        esplits; et.
-        + left. apply plus_one. econs.
-          { instantiate (1:= modsem skenv_link tt). econs; ss; et.
-            - right.
-              unfold load_modsems in *. rewrite in_map_iff. unfold flip. esplits; et; cycle 1.
-              { rewrite in_app_iff. ss. et. }
-              ss.
-            - instantiate (1:= if_sig).
-              eapply genv_sim; et. esplits; et. rr; des; ss; et.
-          }
-          econs; et.
-          eapply genv_sim; et. esplits; et. rr; des; ss; et. des; clarify; et.
-        + right. eapply CIH. instantiate (1:= i.(Int.intval)). econs; et.
-          rewrite cons_app with (xhd := {| Frame.ms := flip Mod.modsem skenv_link x; Frame.st := st_init |}).
-          econs 3.
-          { et. }
-          { refl. }
-          { ss. des; clarify; ss; inv INIT. econs. et. }
-          destruct args; ss. clarify.
-          des; ss; clarify.
-          * inv INIT; ss; clarify. econs; et. refl.
-          * inv INIT; ss; clarify. econs; et. refl.
-    - (* Sem.State *)
+    - (* call *)
       inv STK.
-      + pfold. left. right. econs; et.
-        econs; et; cycle 1.
-        { ss. i. inv FINALSRC; ss. }
-        i. ss. des_ifs. inv STEPSRC.
-      + pfold. right. econs; et.
-        { ss. i. inv FINALTGT; ss. inv TAIL; ss; cycle 1.
-          { destruct hds_tgt, tail_tgt; ss. inv TGT; ss. }
-          esplits; et.
-          { apply star_refl. }
-          econs; ss; et.
-        }
+      + (* ctx *)
+        pfold. right. econs; et.
+        { i; ss. des_ifs. inv FINALTGT. }
         i.
+        admit "ctx".
+      + (* focus-call *)
+        pfold. left; right. econs; et.
         econs; et; cycle 1.
-        { ss. i. specialize (SAFESRC _ (star_refl _ _ _ _)). des.
-          - left. inv SAFESRC. inv TAIL. esplits; et. econs; et.
-          - right. des_ifs. inv SAFESRC; inv TAIL; try (by esplits; et; econs; et).
-        }
-        i. ss. des_ifs. inv STEPTGT; ss.
-        * esplits; et.
-          { left. apply plus_one. econs; et. }
-          right. eapply CIH; et. econs; et. econs; et.
-        * esplits; et.
-          { left. apply plus_one. econs; et. }
-          right. eapply CIH; et. econs; et. econs; et.
-        * inv TAIL.
-          -- esplits; et.
-             { left. apply plus_one. econs 4; et. }
-             right. eapply CIH; et. econs; et. econs; et.
-          -- esplits; et.
-             { left. apply plus_one. econs 4; et. }
-             right. eapply CIH; et. econs; et. econs; et.
-          econs; et.
-      inv MSFIND. ss. des; clarify.
-      { (* system *)
-        inv INIT. esplits; eauto.
-        + left. esplits; eauto; cycle 1.
-          { admit "ez - semprops receptive". }
-          apply plus_one.
-          econs; et.
-          { admit "ez - semprops determinate". }
-          ss. des_ifs. econs; et.
-          { econs; ss; et. }
-          econs; et.
-        + right. eapply CIH; et. econs; et. econs; et.
-      }
-      unfold load_modsems in *.
-      rewrite in_map_iff in *. des. clarify. rewrite in_app_iff in *. des; clarify.
-      { (* ctx *)
-        esplits; eauto.
-        + left. esplits; eauto; cycle 1.
-          { admit "ez - semprops receptive". }
-          apply plus_one.
-          econs; et.
-          { admit "ez - semprops determinate". }
-          ss. des_ifs. econs; et.
-          { econs; ss; et. }
-          econs; et.
-        + right. eapply CIH; et. econs; et. econs; et.
-        +
-      }
-    -
-    admit "".
+        { i; ss. inv FINALSRC. }
+        i.
+        admit "todo".
+      + (* focus-return *)
+        ss.
+    - (* normal *)
+      inv STK.
+      + (* ctx *)
+        admit "ctx".
+      + (* focus-call *)
+        pfold. left; right. econs; et.
+        (* econs; et; cycle 1. *)
+        (* { i; ss. inv FINALSRC. ss. inv FINAL. } *)
+        (* i. ss. des_ifs. *)
+        (* assert(tr = E0). *)
+        (* { inv STEPSRC; clarify. ss. inv STEP. ss. } *)
+        (* clarify. *)
+        destruct (classic (cur = Int.zero)).
+        * clarify.
+          unsguard TGT. des; clarify.
+          { ss.
+            rewrite int_zero_intval in *.
+            econs 1; et; cycle 1.
+            { i; ss. inv FINALSRC. ss. inv FINAL. }
+            i. inv STEPSRC; ss; cycle 1.
+            { inv FINAL. }
+            inv STEP.
+            esplits; et.
+            - left. esplits; eauto.
+              + apply plus_one. econs; eauto.
+                { admit "ez - determinate". }
+                ss. des_ifs. rpapply step_internal. ss.
+              + { admit "ez - receptive". }
+            - right. eapply CIH. econs 2; eauto. econs 3; eauto.
+              + ss.
+              + unfold Frame.update_st. ss. unfold __GUARD__. rewrite sum_recurse. des_ifs; et.
+              + rewrite int_zero_intval. lia.
+          }
+          { ss.
+            rewrite int_zero_intval in *.
+            econs 1; et; cycle 1.
+            { i; ss. inv FINALSRC. ss. inv FINAL. }
+            i. inv STEPSRC; ss; cycle 1.
+            { inv FINAL. }
+            inv STEP.
+            esplits; et.
+            - left. esplits; eauto.
+              + apply plus_one. econs; eauto.
+                { admit "ez - determinate". }
+                ss. des_ifs. rpapply step_internal. ss.
+              + { admit "ez - receptive". }
+            - right. eapply CIH. econs 2; eauto. econs 3; eauto.
+              + ss.
+              + unfold Frame.update_st. ss. unfold __GUARD__. rewrite sum_recurse. des_ifs; et.
+              + rewrite int_zero_intval. lia.
+          }
+        * unsguard TGT. des; clarify.
+          {
+            econs 2; et.
+            - esplits; et.
+              + eapply plus_two with (t1 := E0) (t2 := E0); ss.
+                * econs; eauto.
+                  { admit "ez - determinate". }
+                  ss. des_ifs. econs; eauto. ss. econs; eauto.
+                  { admit "ez - genv g_id some". }
+                  ii. destruct cur; ss. clarify. apply H.
+                  Local Transparent Int.repr.
+                  eapply eta.
+                  Local Opaque Int.repr.
+                  ss.
+                * econs; eauto.
+                  { admit "ez - determinate". }
+                  ss. des_ifs. econs; eauto.
+                  { ss. instantiate (1:= MutrecBspec.modsem skenv_link tt). econs; ss; eauto.
+                    - right. unfold load_modsems. rewrite in_map_iff. esplits; et; cycle 1.
+                      + rewrite in_app_iff. right. ss. right; et.
+                      + ss.
+                    - des_ifs. instantiate (2 := g_id). admit "ez - genv g_id some".
+                  }
+                  ss. econs; ss; eauto.
+                  admit "ez - genv g_id some".
+              + instantiate (1:= Int.intval cur - 1). rr. esplits; try lia. admit "by definition".
+            - right. eapply CIH. econs; eauto.
+              assert(ARITH: Int.intval (Int.sub cur (Int.repr 1)) = Int.intval cur - 1).
+              { admit "ez - arithmetic. it does not underflow". }
+              replace
+                ({| Frame.ms := MutrecBspec.modsem skenv_link tt; Frame.st := MutrecBspec.Callstate (Int.sub cur (Int.repr 1)) m |}
+                   :: {| Frame.ms := MutrecAspec.modsem skenv_link tt; Frame.st := MutrecAspec.Callstate cur m |} :: hds_tgt ++ ctx_stk) with
+                 ({| Frame.ms := MutrecBspec.modsem skenv_link tt; Frame.st := MutrecBspec.Callstate (Int.sub cur (Int.repr 1)) m |}
+                   :: ({| Frame.ms := MutrecAspec.modsem skenv_link tt; Frame.st := MutrecAspec.Callstate cur m |} :: hds_tgt) ++ ctx_stk) by ss.
+              econs 2.
+              + refl.
+              + unfold __GUARD__. ss. eauto.
+              + rewrite ARITH. lia.
+              + rewrite int_sub_add.
+                econs; eauto.
+                (* left. rpapply FOCUS. f_equal. rewrite Int.sub_add_opp. rewrite Int.add_assoc. *)
+                (* rewrite Int.add_commut with (y := Int.one). *)
+                (* rewrite Int.add_neg_zero. rewrite Int.add_zero. ss. *)
+                (* admit "". *)
+                (* admit "". *)
+              + rewrite ARITH. lia.
+          }
+          {
+            econs 2; et.
+            - esplits; et.
+              + eapply plus_two with (t1 := E0) (t2 := E0); ss.
+                * econs; eauto.
+                  { admit "ez - determinate". }
+                  ss. des_ifs. econs; eauto. ss. econs; eauto.
+                  { admit "ez - genv f_id some". }
+                  ii. destruct cur; ss. clarify. apply H.
+                  Local Transparent Int.repr.
+                  eapply eta.
+                  Local Opaque Int.repr.
+                  ss.
+                * econs; eauto.
+                  { admit "ez - determinate". }
+                  ss. des_ifs. econs; eauto.
+                  { ss. instantiate (1:= MutrecAspec.modsem skenv_link tt). econs; ss; eauto.
+                    - right. unfold load_modsems. rewrite in_map_iff. esplits; et; cycle 1.
+                      + rewrite in_app_iff. right. ss. left; et.
+                      + ss.
+                    - des_ifs. instantiate (2 := f_id). admit "ez - genv f_id some".
+                  }
+                  ss. econs; ss; eauto.
+                  admit "ez - genv f_id some".
+              + instantiate (1:= Int.intval cur - 1). split; try lia. admit "by definition".
+            - right. eapply CIH. econs; eauto.
+              assert(ARITH: Int.intval (Int.sub cur (Int.repr 1)) = Int.intval cur - 1).
+              { admit "ez - arithmetic. it does not underflow". }
+              replace
+                ({| Frame.ms := MutrecAspec.modsem skenv_link tt; Frame.st := MutrecAspec.Callstate (Int.sub cur (Int.repr 1)) m |}
+                   :: {| Frame.ms := MutrecBspec.modsem skenv_link tt; Frame.st := MutrecBspec.Callstate cur m |} :: hds_tgt ++ ctx_stk) with
+                  ({| Frame.ms := MutrecAspec.modsem skenv_link tt; Frame.st := MutrecAspec.Callstate (Int.sub cur (Int.repr 1)) m |}
+                     :: ({| Frame.ms := MutrecBspec.modsem skenv_link tt; Frame.st := MutrecBspec.Callstate cur m |} :: hds_tgt) ++ ctx_stk) by ss.
+              econs 2.
+              + refl.
+              + unfold __GUARD__. ss. eauto.
+              + rewrite ARITH. lia.
+              + rewrite int_sub_add.
+                econs; eauto.
+                (* left. rpapply FOCUS. f_equal. rewrite Int.sub_add_opp. rewrite Int.add_assoc. *)
+                (* rewrite Int.add_commut with (y := Int.one). *)
+                (* rewrite Int.add_neg_zero. rewrite Int.add_zero. ss. *)
+                (* admit "". *)
+                (* admit "". *)
+              + rewrite ARITH. lia.
+          }
+      + (* focus - return *)
+        destruct (classic (cur = max)).
+        * clarify. exploit match_focus_over_nil; eauto. i; clarify.
+          pfold. right. econs; eauto.
+          { i. ss. inv FINALTGT.
+            unsguard TGT. des; clarify; ss.
+            - inv FINAL. ss. clarify. esplits; eauto. { apply star_refl. } econs; ss; eauto.
+            - inv FINAL. ss. clarify. esplits; eauto. { apply star_refl. } econs; ss; eauto.
+          }
+          i. econs; eauto; cycle 1.
+          { i. specialize (SAFESRC _ (star_refl _ _ _ _)). desH SAFESRC; ss.
+            - inv SAFESRC; ss. inv FINAL. ss. clarify. left.
+              unsguard TGT. des; clarify.
+              { esplits; eauto. econs; ss; eauto. }
+              { esplits; eauto. econs; ss; eauto. }
+            - des_ifs. right. inv SAFESRC; ss.
+              { inv STEP. }
+              inv FINAL. esplits; eauto. econs 4; eauto.
+              unsguard TGT. des; clarify.
+          }
+          i. ss. des_ifs. inv STEPTGT; ss.
+          { unsguard TGT. des; clarify; inv AT. }
+          { unsguard TGT. des; clarify; inv STEP. }
+          esplits; eauto.
+          -- left. apply plus_one. econs 4; eauto. ss. unsguard TGT. des; clarify; ss; inv FINAL; econs; eauto.
+          -- right. eapply CIH. econs; eauto. econs; eauto.
+        * pfold. left. right. econs; eauto.
+          (* TODO: ---------> we can remove redundancy. current match_states include A-A-B-A-B-A... or B-B-A-B-A-B ... *)
+          unsguard TGT. des; clarify.
+          { inv FOCUS; ss.
+            { exfalso. admit "ez - arithmetic". }
+            {
+              econs 2; eauto.
+              - esplits; eauto.
+                + apply plus_one. econs; eauto.
+                  { admit "ez - determinate". }
+                  ss. des_ifs.
+                  econs 4; ss; eauto.
+                  econs; ss; eauto.
+                  rewrite Int.add_commut.
+                  rewrite Int.sub_add_l. rewrite Int.sub_idem. rewrite Int.add_zero_l. ss.
+                + instantiate (1:= Int.intval max - Int.intval cur - 1). split; try lia.
+              - right. eapply CIH; eauto. unfold Frame.update_st. ss. econs; eauto. econs 3; ss.
+                + unfold __GUARD__. eauto.
+                + admit "ez - arithmetic".
+                + ss.
+                + admit "ez - arithmetic. no overflow".
+            }
+            {
+              econs 2; eauto.
+              - esplits; eauto.
+                + apply plus_one. econs; eauto.
+                  { admit "ez - determinate". }
+                  ss. des_ifs.
+                  econs 4; ss; eauto.
+                  econs; ss; eauto.
+                  rewrite Int.add_commut.
+                  rewrite Int.sub_add_l. rewrite Int.sub_idem. rewrite Int.add_zero_l. ss.
+                + instantiate (1:= Int.intval max - Int.intval cur - 1). split; try lia.
+              - right. eapply CIH; eauto. unfold Frame.update_st. ss. econs; eauto. econs 3; ss.
+                + unfold __GUARD__. eauto.
+                + admit "ez - arithmetic".
+                + ss.
+                + admit "ez - arithmetic. no overflow".
+            }
+          }
+          { inv FOCUS; ss.
+            { exfalso. admit "ez - arithmetic". }
+            {
+              econs 2; eauto.
+              - esplits; eauto.
+                + apply plus_one. econs; eauto.
+                  { admit "ez - determinate". }
+                  ss. des_ifs.
+                  econs 4; ss; eauto.
+                  econs; ss; eauto.
+                  rewrite Int.add_commut.
+                  rewrite Int.sub_add_l. rewrite Int.sub_idem. rewrite Int.add_zero_l. ss.
+                + instantiate (1:= Int.intval max - Int.intval cur - 1). split; try lia.
+              - right. eapply CIH; eauto. unfold Frame.update_st. ss. econs; eauto. econs 3; ss.
+                + unfold __GUARD__. eauto.
+                + admit "ez - arithmetic".
+                + ss.
+                + admit "ez - arithmetic. no overflow".
+            }
+            {
+              econs 2; eauto.
+              - esplits; eauto.
+                + apply plus_one. econs; eauto.
+                  { admit "ez - determinate". }
+                  ss. des_ifs.
+                  econs 4; ss; eauto.
+                  econs; ss; eauto.
+                  rewrite Int.add_commut.
+                  rewrite Int.sub_add_l. rewrite Int.sub_idem. rewrite Int.add_zero_l. ss.
+                + instantiate (1:= Int.intval max - Int.intval cur - 1). split; try lia.
+              - right. eapply CIH; eauto. unfold Frame.update_st. ss. econs; eauto. econs 3; ss.
+                + unfold __GUARD__. eauto.
+                + admit "ez - arithmetic".
+                + ss.
+                + admit "ez - arithmetic. no overflow".
+            }
+          }
+  Unshelve.
+    all: admit "abc".
   Qed.
 
 End LXSIM.
@@ -434,9 +483,6 @@ End LXSIM.
 Theorem mutrecABcorrect
         ctx
   :
-    (* (<<REFINE: improves (Sem.sem ([(MutrecABspec.module)] ++ ctx)) *)
-    (*                     (Sem.sem ([(MutrecAspec.module) ; (MutrecBspec.module)] ++ ctx)) *)
-    (*                     >>) *)
     (<<REFINE: improves (Sem.sem (ctx ++ [(MutrecABspec.module)]))
                         (Sem.sem (ctx ++ [(MutrecAspec.module) ; (MutrecBspec.module)]))
                         >>)
@@ -446,7 +492,7 @@ Proof.
   eapply mixed_to_backward_simulation.
   econs; eauto.
   econs; swap 2 3.
-  { apply lt_wf. }
+  { instantiate (1:= Zwf.Zwf 0%Z). eapply Zwf.Zwf_well_founded. }
   { i; des. ss. inv SAFESRC. rewrite INITSK.
     ss. rewrite link_sk_same. des_ifs.
   }
@@ -463,328 +509,6 @@ Proof.
         * eapply wf_module_Bspec; et.
     - i; ss. inv INIT0. inv INIT1. clarify.
   }
-  eapply match_states_xsim; et.
-  econs; et. econs; et.
+  eapply match_states_xsim; eauto.
+  econs; eauto. econs; eauto.
 Qed.
-
-
-(* Inductive match_states_internal: MutrecABspec.state -> Clight.state -> Prop := *)
-(* | match_callstate_nonzero *)
-(*     i m_src m_tgt *)
-(*     fptr *)
-(*     (* targs tres cconv *) *)
-(*     (FINDF: Genv.find_funct (Smallstep.globalenv (modsem2 skenv_link prog)) fptr = Some (Internal func_f)) *)
-(*   : *)
-(*     match_states_internal (Callstate i m_src) (Clight.Callstate fptr (Tfunction (* targs tres cconv) *) *)
-(*                                                                         (Tcons tint Tnil) tint cc_default) *)
-(*                                                                 [Vint i] Kstop m_tgt) *)
-(* | match_returnstate *)
-(*     i m_src m_tgt *)
-(*   : *)
-(*     match_states_internal (Returnstate i m_src) (Clight.Returnstate (Vint i) Kstop m_tgt) *)
-(* . *)
-
-(* Inductive match_states (sm_init: SimMem.t) *)
-(*           (idx: nat) (st_src0: MutrecAspec.state) (st_tgt0: Clight.state) (sm0: SimMem.t): Prop := *)
-(* | match_states_intro *)
-(*     (MATCHST: match_states_internal st_src0 st_tgt0) *)
-(*     (MCOMPATSRC: st_src0.(get_mem) = sm0.(SimMem.src)) *)
-(*     (MCOMPATTGT: st_tgt0.(ClightC.get_mem) = sm0.(SimMem.tgt)) *)
-(*     (MWF: SimMem.wf sm0) *)
-(*     (IDX: (idx > 3)%nat) *)
-(* . *)
-
-Theorem make_match_genvs :
-  SimSymbId.sim_skenv (SkEnv.project skenv_link md_src.(Mod.sk)) (SkEnv.project skenv_link md_tgt.(Mod.sk)) ->
-  Genv.match_genvs (match_globdef (fun _ => eq) eq tt) ge tge.
-Proof.
-  subst_locals. ss. ii.
-  eapply SimSymbId.sim_skenv_revive; eauto.
-  admit "ez - reflexivity".
-Qed.
-
-Lemma g_blk_exists
-  :
-    exists g_blk,
-      (<<FINDG: Genv.find_symbol
-                  (SkEnv.revive (SkEnv.project skenv_link (CSk.of_program signature_of_function prog)) prog)
-                  g_id = Some g_blk>>)
-      /\
-      (<<FINDG: Genv.find_funct_ptr
-                  (SkEnv.revive (SkEnv.project skenv_link (CSk.of_program signature_of_function prog)) prog)
-                  g_blk = None>>)
-      /\
-      (<<FINDG: exists skd, Genv.find_funct_ptr skenv_link g_blk = Some skd /\
-                            signature_of_type (Tcons tint Tnil) tint cc_default = SkEnv.get_sig skd>>)
-.
-Proof.
-  exploit (prog_defmap_norepet prog g_id); eauto.
-  { unfold prog_defs_names. ss. repeat (econs; eauto). ii; ss; des; ss. }
-  { ss. eauto. }
-  intro T; des.
-  exploit SkEnv.project_impl_spec; eauto. intro PROJ.
-  assert(PREC: SkEnv.genv_precise
-                 (SkEnv.revive (SkEnv.project skenv_link (CSk.of_program signature_of_function prog)) prog)
-                 prog).
-  { eapply CSkEnv.project_revive_precise; ss; et. }
-  inv PREC.
-  exploit (P2GE g_id); eauto. i; des. des_ifs.
-  rename b into g_blk.
-  eexists. splits; et.
-  { unfold Genv.find_funct_ptr. des_ifs. }
-  (* exploit (@SkEnv.project_revive_precise _ _ skenv_link); eauto. *)
-  { inv INCLSRC.
-    exploit (CSk.of_program_prog_defmap prog signature_of_function); et. rewrite T. intro S.
-
-    remember ((prog_defmap (CSk.of_program signature_of_function prog)) ! g_id) as U in *.
-    destruct U eqn:V; try (by ss). inv S. inv H1.
-
-    exploit DEFS; eauto. i; des.
-    assert(blk = g_blk).
-    { inv PROJ. exploit SYMBKEEP; et.
-      - instantiate (1:= g_id). unfold defs. des_sumbool. ss. et.
-      - i. rewrite SYMB0 in *. clear - SYMB H. unfold SkEnv.revive in *. rewrite Genv_map_defs_symb in *. ss.
-        rewrite SYMB in *. des. clarify.
-    }
-    clarify. inv MATCH.
-    esplits; eauto.
-    - unfold Genv.find_funct_ptr. rewrite DEF0. et.
-    - ss. des_ifs. clear - H1. inv H1; ss.
-  }
-Qed.
-
-Lemma match_states_lxsim
-      sm_init idx st_src0 st_tgt0 sm0
-      (MATCH: match_states sm_init idx st_src0 st_tgt0 sm0)
-  :
-    <<XSIM: lxsim (md_src skenv_link) (md_tgt skenv_link)
-                  (fun st => exists su m_init, SoundTop.sound_state su m_init st)
-                  sm_init (Ord.lift_idx lt_wf idx) st_src0 st_tgt0 sm0>>
-.
-Proof.
-  revert_until tge.
-  pcofix CIH.
-  i.
-  pfold.
-  generalize g_blk_exists; et. i; des.
-  inv MATCH. ss. inv MATCHST; ss; clarify.
-  - (* call *)
-    destruct (classic (i = Int.zero)).
-    + (* zero *)
-      clarify.
-      econs 1. i; des.
-      econs 1; cycle 2.
-      { admit "ez - spec is receptive". }
-      { split; ii; rr in H; inv H; inv H0; ss. }
-      i. ss. inv STEPSRC.
-      esplits; eauto.
-      * left.
-        eapply plus_left with (t1 := E0) (t2 := E0); ss.
-        { econs; eauto.
-          { eapply modsem2_determinate; eauto. }
-          econs; eauto.
-          econs; ss; eauto; try (by repeat (econs; ss; eauto)).
-          unfold _x. unfold _t'1. rr. ii; ss. des; ss. clarify.
-        }
-
-        eapply star_left with (t1 := E0) (t2 := E0); ss.
-        { econs; eauto.
-          { eapply modsem2_determinate; eauto. }
-          econs; eauto.
-        }
-
-        eapply star_left with (t1 := E0) (t2 := E0); ss.
-        { econs; eauto.
-          { eapply modsem2_determinate; eauto. }
-          econs; eauto.
-          - repeat econs; et.
-          - ss.
-        }
-
-        eapply star_left with (t1 := E0) (t2 := E0); ss.
-        { econs; eauto.
-          { eapply modsem2_determinate; eauto. }
-          econs; eauto.
-          - repeat econs; et.
-          - ss.
-          - ss.
-        }
-
-        apply star_refl.
-      (* * refl. *)
-      * right. eapply CIH. econs; ss; eauto. econs; eauto.
-    + (* nonzero *)
-      econs.
-      i; des.
-      econs 2; eauto.
-      * esplits; cycle 1.
-        { eapply Ord.lift_idx_spec. instantiate (1:= 2%nat). lia. }
-
-        eapply plus_left with (t1 := E0) (t2 := E0); ss.
-        { econs; eauto.
-          { eapply modsem2_determinate; eauto. }
-          econs; eauto.
-          econs; ss; eauto; try (by repeat (econs; ss; eauto)).
-          unfold _x. unfold _t'1. rr. ii; ss. des; ss. clarify.
-        }
-        
-        eapply star_left with (t1 := E0) (t2 := E0); ss.
-        { econs; eauto.
-          { eapply modsem2_determinate; eauto. }
-          econs; eauto.
-        }
-
-        eapply star_left with (t1 := E0) (t2 := E0); ss.
-        { econs; eauto.
-          { eapply modsem2_determinate; eauto. }
-          econs; eauto.
-          - repeat econs; et.
-          - ss. rewrite Int.eq_false; ss.
-        }
-
-        eapply star_left with (t1 := E0) (t2 := E0); ss.
-        { econs; eauto.
-          { eapply modsem2_determinate; eauto. }
-          econs; eauto.
-        }
-
-        eapply star_left with (t1 := E0) (t2 := E0); ss.
-        { econs; eauto.
-          { eapply modsem2_determinate; eauto. }
-          econs; eauto.
-        }
-
-        eapply star_left with (t1 := E0) (t2 := E0); ss.
-        { econs; eauto.
-          { eapply modsem2_determinate; eauto. }
-          econs; eauto; swap 1 2.
-          - econs.
-            + eapply eval_Evar_global; ss. et.
-            + econs 2; et.
-          - unfold Cop.classify_fun. ss.
-          - repeat econs; ss; et.
-        }
-
-        apply star_refl.
-      * left. pfold. econs 3; et.
-        { rr. esplits; eauto. ss. econs; et. ii. destruct i; ss. clarify. apply H. unfold Int.zero.
-          Local Transparent Int.repr.
-          unfold Int.repr.
-          Local Opaque Int.repr.
-          ss. apply eta; ss.
-        }
-        ii; des.
-        inv ATSRC. ss; clarify.
-        destruct sm0; ss. clarify.
-        unfold Clight.fundef in *.
-        rewrite FINDG in *. clarify.
-        eexists (Args.mk _ [Vint (Int.sub i (Int.repr 1))] _), (SimMemId.mk _ _).
-        esplits; ss; eauto.
-        { econs; ss; eauto. }
-        i. inv AFTERSRC. destruct retv_src, retv_tgt; ss. clarify. destruct sm_ret; ss. inv SIMRETV; ss; clarify.
-        esplits; eauto.
-        { econs; eauto. }
-        instantiate (2:= (Ord.lift_idx lt_wf 15%nat)).
-        left. pfold. econs; eauto. i; des. econs 2; eauto.
-        {
-          esplits; eauto; cycle 1.
-          { instantiate (1:= (Ord.lift_idx lt_wf 14%nat)). eapply Ord.lift_idx_spec; et. }
-
-          eapply plus_left with (t1 := E0) (t2 := E0); ss.
-          { econs; eauto.
-            { eapply modsem2_determinate; eauto. }
-            econs; eauto.
-          }
-          
-          eapply star_left with (t1 := E0) (t2 := E0); ss.
-          { econs; eauto.
-            { eapply modsem2_determinate; eauto. }
-            econs; eauto.
-          }
-
-          eapply star_left with (t1 := E0) (t2 := E0); ss.
-          { econs; eauto.
-            { eapply modsem2_determinate; eauto. }
-            econs; ss; eauto.
-            - repeat (econs; ss; eauto).
-              + unfold typify. des_ifs.
-              + ss.
-            - ss.
-          }
-
-          eapply star_refl.
-        }
-        
-        right. eapply CIH. instantiate (1:= SimMemId.mk _ _).
-        econs; ss; eauto; try lia.
-        rewrite sum_recurse. des_ifs.
-        { rewrite Z.eqb_eq in *. lia. }
-        replace (Int.sub (Int.add (sum (Int.sub i Int.one)) i) (Int.repr 1)) with
-            (Int.add (sum (Int.sub i Int.one)) (Int.sub i Int.one)); cycle 1.
-        { abstr (sum (Int.sub i Int.one)) z. rewrite ! Int.sub_add_opp.
-          rewrite Int.add_assoc. ss. }
-        econs; eauto.
-  - (* return *)
-    econs 4; ss; eauto.
-Unshelve.
-  all: ss.
-Qed.
-
-Theorem sim_modsem
-  :
-    ModSemPair.sim msp
-.
-Proof.
-  econs; eauto.
-  { eapply SoundTop.sound_state_local_preservation. }
-  i. ss. esplits; eauto; cycle 1.
-  { (* init progress *)
-    i.
-    des. inv SAFESRC.
-    inv SIMARGS; ss.
-    (* hexploit (SimMemInjC.skenv_inject_revive prog); et. { apply SIMSKENV. } intro SIMSKENV0; des. *)
-    exploit make_match_genvs; eauto. { apply SIMSKENV. } intro SIMGE.
-
-    (* hexploit (@fsim_external_inject_eq); try apply FINDF; eauto. clear FPTR. intro FPTR. *)
-
-    esplits; eauto. econs; eauto.
-    + rewrite <- FPTR. eauto.
-    + instantiate (1:= [Vint i]). rewrite VS in *. inv VALS. econs; ss.
-      cbn. unfold typify. des_ifs; ss.
-  }
-  (* init bsim *)
-  ii.
-  destruct sm_arg; ss. clarify.
-  clear MFUTURE.
-  inv SIMARGS; ss. clarify.
-  inv INITTGT.
-  (* hexploit (SimMemInjC.skenv_inject_revive prog); et. { apply SIMSKENV. } intro SIMSKENV0; des. *)
-  exploit make_match_genvs; eauto. { apply SIMSKENV. } intro SIMGE. des.
-  eexists. eexists (SimMemId.mk _ _).
-  esplits; eauto.
-  + eapply match_states_lxsim.
-    econs; ss; eauto; cycle 1.
-    { inv SAFESRC. ss. }
-
-    inv SAFESRC. destruct args_src, args_tgt; ss. clarify.
-    assert(tvs = [Vint i]).
-    {
-      unfold signature_of_function in TYP. ss.
-      inv TYP. ss. cbn. unfold typify. des_ifs; ss.
-    } clarify.
-    econs; eauto.
-Unshelve.
-  all: try (ss; econs).
-Qed.
-
-End SIMMODSEM.
-
-Theorem sim_mod
-  :
-    ModPair.sim (ModPair.mk (MutrecAspec.module prog) (ClightC.module2 prog) tt)
-.
-Proof.
-  econs; ss.
-  - ii. inv SIMSKENVLINK. eapply sim_modsem; eauto.
-Qed.
-
